theories/Eq/UpToTausH.v
@@ -1,0 +1,1004 @@
+(* Equivalence up to taus *)
+(* We consider tau as an "internal step", that should not be
+   visible to the outside world, so adding or removing [Tau]
+   constructors from an itree should produce an equivalent itree.
+
+   We must be careful because there may be infinite sequences of
+   taus (i.e., [spin]). Here we shall only allow inserting finitely
+   many taus between any two visible steps ([Ret] or [Vis]), so that
+   [spin] is only related to itself. The main consequence of this
+   choice is that equivalence up to taus is an equivalence relation.
+ *)
+
+(* TODO:
+   - relate to Eq.Eq.eq_itree
+   - prove monad laws (see [eutt_bind_bind_fail])
+   - make [eutt] easier to work with ([eutt_bind] is already a mess)
+ *)
+
+Require Import Paco.paco.
+
+From Coq Require Import
+     Program
+     Lia
+     Classes.RelationClasses
+     Classes.Morphisms
+     Setoids.Setoid
+     Relations.Relations
+     Logic.JMeq Logic.EqdepFacts.
+
+From ITree Require Import Core Eq.Eq.
+
+Local Open Scope itree.
+
+(* [notau t] holds when [t] does not start with a [Tau]. *)
+Definition notauF {E R I} (t : itreeF E R I) : Prop :=
+  match t with
+  | TauF _ => False
+  | _ => True
+  end.
+Arguments notauF [E R I] t.
+
+Notation notau t := (notauF (observe t)).
+
+Section EUTT.
+
+Context {E : Type -> Type} {R : Type}.
+
+(* Equivalence between visible steps of computation (i.e., [Vis] or
+   [Ret], parameterized by a relation [eutt] between continuations
+   in the [Vis] case. *)
+Variant eq_notauF {I} (eutt : relation I)
+: relation (itreeF E R I) :=
+| Eutt_ret : forall r, eq_notauF eutt (RetF r) (RetF r)
+| Eutt_vis : forall u (e : E u) k1 k2,
+    (forall x, eutt (k1 x) (k2 x)) ->
+    eq_notauF eutt (VisF e k1) (VisF e k2).
+Hint Constructors eq_notauF.
+
+Variant eq_notauF' {I} (eutt : relation I)
+: relation (itreeF E R I) :=
+| Eutt_ret' : forall r, eq_notauF' eutt (RetF r) (RetF r)
+| Eutt_vis' : forall {u1 u2} (e1 : E u1) (e2 : E u2) k1 k2,
+    eq_dep _ E _ e1 _ e2 ->
+    (forall x1 x2, JMeq x1 x2 -> eutt (k1 x1) (k2 x2)) ->
+    eq_notauF' eutt (VisF e1 k1) (VisF e2 k2).
+Hint Constructors eq_notauF'.
+
+Lemma eq_notauF_eq_eq_notauF': forall I (eutt : relation I) t s,
+  eq_notauF eutt t s <-> eq_notauF' eutt t s.
+Proof.
+  split; intros EUTT; destruct EUTT; eauto.
+  - econstructor; intros; subst; eauto.
+  - assert (u1 = u2) by (inv H; eauto).
+    subst. apply eq_dep_eq in H. subst. eauto.
+Qed.
+
+(* [untaus t' t] holds when [t = Tau (... Tau t' ...)]:
+   [t] steps to [t'] by "peeling off" a finite number of [Tau].
+   "Peel off" means to remove only taus at the root of the tree,
+   not any behind a [Vis] step). *)
+Inductive untausF : relation (itreeF E R _) :=
+| NoTau ot0 : untausF ot0 ot0
+| OneTau ot t' ot0 (OBS: TauF t' = ot) (TAUS: untausF (observe t') ot0): untausF ot ot0
+.
+Hint Constructors untausF.
+
+Definition unalltausF ot ot0 := untausF ot ot0 /\ notauF ot0.
+Hint Unfold unalltausF.
+
+
+(* [finite_taus t] holds when [t] has a finite number of taus
+   to peel. *)
+Definition finite_tausF ot : Prop := exists ot', unalltausF ot ot'.
+Hint Unfold finite_tausF.
+
+(* [eutt_ eutt t1 t2] means that, if [t1] or [t2] ever takes a
+   visible step ([Vis] or [Ret]), then the other takes the same
+   step, and the subsequent continuations (in the [Vis] case) are
+   related by [eutt]. In particular, [(t1 = spin)%eq_itree] if
+   and only if [(t2 = spin)%eq_itree]. Note also that in that
+   case, the parameter [eutt] is irrelevant.
+
+   This is the relation we will take a fixpoint of. *)
+Inductive euttF (eutt : relation (itree E R)) (ot1 ot2: itreeF E R (itree E R)) : Prop :=
+| euttF_ (FIN: finite_tausF ot1 <-> finite_tausF ot2)
+         (EQV: forall ot1' ot2'
+                  (UNTAUS1: unalltausF ot1 ot1')
+                  (UNTAUS2: unalltausF ot2 ot2'),
+               eq_notauF eutt ot1' ot2')
+.
+Hint Constructors euttF.
+
+Definition eutt_ (eutt : relation (itree E R)) (t1 t2 : itree E R) : Prop :=
+  euttF eutt (observe t1) (observe t2).
+Hint Unfold eutt_.
+
+(* Paco takes the greatest fixpoints of monotone relations. *)
+
+Lemma monotone_eq_notauF : forall I (r r' : relation I) x1 x2
+      (IN: eq_notauF r x1 x2)
+      (LE: r <2= r'),
+    eq_notauF r' x1 x2.
+Proof. pmonauto. Qed.
+Hint Resolve monotone_eq_notauF.
+
+(* [eutt_] is monotone. *)
+Lemma monotone_eutt_ : monotone2 eutt_.
+Proof. pmonauto. Qed.
+Hint Resolve monotone_eutt_ : paco.
+
+(* We now take the greatest fixpoint of [eutt_]. *)
+
+(* Equivalence Up To Taus.
+
+   [eutt t1 t2]: [t1] is equivalent to [t2] up to taus. *)
+Definition eutt : relation (itree E R) := paco2 eutt_ bot2.
+
+Global Arguments eutt t1%itree t2%itree.
+
+Infix "~~" := eutt (at level 70) : itree_scope.
+
+(* Lemmas about the auxiliary relations. *)
+
+(* Many have a name [X_Y] to represent an implication
+   [X _ -> Y _] (possibly with more arguments on either side). *)
+
+Lemma untaus_all ot ot' :
+  untausF ot ot' -> notauF ot' -> unalltausF ot ot'.
+Proof. induction 1; eauto. Qed.
+
+Lemma unalltaus_notau ot ot' : unalltausF ot ot' -> notauF ot'.
+Proof. intros. induction H; eauto. Qed.
+
+Lemma notau_tau I (ot : itreeF E R I) (t0 : I)
+  (NOTAU : notauF ot)
+  (OBS: TauF t0 = ot): False.
+Proof. subst. auto. Qed.
+Hint Resolve notau_tau.
+
+Lemma notau_ret I (ot: itreeF E R I) r (OBS: RetF r = ot) : notauF ot.
+Proof. subst. red. eauto. Qed.
+Hint Resolve notau_ret.
+
+Lemma notau_vis I (ot : itreeF E R I) u (e: E u) k (OBS: VisF e k = ot) : @notauF E R I ot.
+Proof. intros. subst. red. eauto. Qed.
+Hint Resolve notau_vis.
+
+(* If [t] does not start with [Tau], removing all [Tau] does
+   nothing. Can be thought of as [notau_unalltaus] composed with
+   [unalltaus_injective] (below). *)
+Lemma unalltaus_notau_id ot ot' :
+  unalltausF ot ot' -> notauF ot -> ot = ot'.
+Proof.
+  intros [[ | ]] ?; eauto. exfalso; eauto.
+Qed.
+
+(* There is only one way to peel off all taus. *)
+Lemma unalltaus_injective ot ot1 ot2 :
+    unalltausF ot ot1 -> unalltausF ot ot2 -> ot1 = ot2.
+Proof.
+  intros [Huntaus Hnotau]. revert ot2 Hnotau.
+  induction Huntaus; intros; eauto using unalltaus_notau_id.
+  eapply IHHuntaus; eauto.
+  destruct H as [Huntaus' Hnotau'].
+  destruct Huntaus'.
+  + exfalso; eauto.
+  + subst. inversion OBS0; subst; eauto.
+Qed.
+
+(* Adding a [Tau] to [t1] then peeling them all off produces
+   the same result as peeling them all off from [t1]. *)
+Lemma unalltaus_tau t ot1 ot2
+    (OBS: TauF t = ot1)
+    (TAUS: unalltausF ot1 ot2):
+  unalltausF (observe t) ot2.
+Proof.
+  destruct TAUS as [Huntaus Hnotau].
+  destruct Huntaus.
+  - exfalso; eauto.
+  - subst; inversion OBS0; subst; eauto.
+Qed.
+
+Lemma unalltaus_tau' t ot1 ot2
+    (OBS: TauF t = ot1)
+    (TAUS: unalltausF (observe t) ot2):
+  unalltausF ot1 ot2.
+Proof.
+  destruct TAUS as [Huntaus Hnotau].
+  subst. eauto.
+Qed.
+
+Lemma notauF_untausF ot1 ot2
+      (NOTAU : notauF ot1)
+      (UNTAUS : untausF ot1 ot2) : ot1 = ot2.
+Proof.
+  destruct UNTAUS; eauto.
+  exfalso; eauto.
+Qed.
+
+Definition untausF_shift (t1 t2 : itree E R) :
+  untausF (TauF t1) (TauF t2) -> untausF (observe t1) (observe t2).
+Proof.
+  intros H.
+  inversion H; subst.
+  { constructor. }
+  clear H.
+  inversion OBS; subst; clear OBS.
+  remember (observe t1) as ot1.
+  remember (TauF t2) as tt2.
+  generalize dependent t1.
+  generalize dependent t2.
+  induction TAUS; intros; subst; econstructor; eauto.
+Qed.
+
+Definition untausF_trans (t1 t2 t3 : itreeF E R _) :
+  untausF t1 t2 -> untausF t2 t3 -> untausF t1 t3.
+Proof.
+  induction 1; auto.
+  subst; econstructor; auto.
+Qed.
+
+Definition untausF_strong_ind
+           (P : itreeF E R _ -> Prop)
+           (ot1 ot2 : itreeF E R _)
+           (Huntaus : untausF ot1 ot2)
+           (Hnotau : notauF ot2)
+           (STEP : forall ot1
+               (Huntaus : untausF ot1 ot2)
+               (IH: forall t1' oti
+                     (NEXT: ot1 = TauF t1')
+                     (UNTAUS: untausF (observe t1') oti),
+                   P oti),
+               P ot1)
+  : P ot1.
+Proof.
+  enough (H : forall oti,
+             untausF ot1 oti ->
+             untausF oti ot2 ->
+             P oti
+         ).
+  { apply H; eauto. }
+  revert STEP.
+  induction Huntaus; intros; subst.
+  - eapply STEP; eauto.
+    intros; subst. dependent destruction H; inv Hnotau.
+  - destruct H0; auto.
+    subst. apply STEP; eauto.
+    intros. inv NEXT.
+    apply IHHuntaus; eauto.
+    + clear -H UNTAUS.
+      remember (TauF t') as ott'. remember (TauF t1') as ott1'.
+      move H at top. revert_until H. induction H; intros; subst.
+      * inv Heqott1'. eauto.
+      * inv Heqott'. dependent destruction H; eauto.
+    + genobs t1' ot1'. revert UNTAUS. clear -Hnotau H0. induction H0; intros.
+      * dependent destruction UNTAUS; eauto.
+        subst. simpobs. inv Hnotau.
+      * subst. dependent destruction UNTAUS; eauto.
+Qed.
+
+(* If [t] does not start with [Tau], then it starts with finitely
+   many [Tau]. *)
+Lemma notau_finite_taus ot : notauF ot -> finite_tausF ot.
+Proof. eauto. Qed.
+
+(* [Vis] and [Ret] start with no taus, of course. *)
+Lemma finite_taus_ret ot (r : R) (OBS: RetF r = ot) : finite_tausF ot.
+Proof. eauto 10. Qed.
+
+Lemma finite_taus_vis {u} ot (e : E u) (k : u -> itree E R) (OBS: VisF e k = ot):
+  finite_tausF ot.
+Proof. eauto 10. Qed.
+
+(* [finite_taus] is preserved by removing or adding one [Tau]. *)
+Lemma finite_taus_tau t':
+  finite_tausF (TauF t') <-> finite_tausF (observe t').
+Proof.
+  split; intros [? [Huntaus Hnotau]]; eauto 10.
+  inv Huntaus.
+  - contradiction.
+  - inv OBS; eauto.
+Qed.
+
+(* (* [finite_taus] is preserved by removing or adding any finite *)
+(*    number of [Tau]. *) *)
+Lemma untaus_finite_taus ot ot':
+    untausF ot ot' -> (finite_tausF ot <-> finite_tausF ot').
+Proof.
+  induction 1; intros; subst.
+  - reflexivity.
+  - erewrite finite_taus_tau; eauto.
+Qed.
+
+(**)
+
+Lemma eq_unalltaus (t1 t2 : itree E R) ot1'
+    (FT: unalltausF (observe t1) ot1')
+    (EQV: t1 ≅ t2) :
+  exists ot2', unalltausF (observe t2) ot2'.
+Proof.
+  genobs t1 ot1. revert t1 Heqot1 t2 EQV.
+  destruct FT as [Huntaus Hnotau].
+  induction Huntaus; intros; punfold EQV; unfold_eq_itree; subst.
+  - eexists. constructor; eauto. inv EQV; simpl; eauto.
+  - inv EQV; simpobs; try inv Heqot1.
+    pclearbot. edestruct IHHuntaus as [? []]; eauto.
+Qed.
+
+Lemma eq_unalltaus_eqF (t s : itree E R) ot'
+    (UNTAUS : unalltausF (observe t) ot')
+    (EQV: t ≅ s) :
+  exists os', unalltausF (observe s) os' /\ eq_itreeF' eq_itree ot' os'.
+Proof.
+  destruct UNTAUS as [Huntaus Hnotau].
+  remember (observe t) as ot. revert s t Heqot EQV.
+  induction Huntaus; intros; punfold EQV; unfold_eq_itree.
+  - eexists (observe s). split.
+    inv EQV; simpobs; eauto.
+    subst; eauto.
+    eapply eq_itreeF'_mono; eauto.
+    intros ? ? [| []]; eauto.
+  - inv EQV; rewrite <- H0 in Heqot; inversion Heqot; subst.
+    destruct REL as [| []].
+    edestruct IHHuntaus as [? [[]]]; eauto 10.
+Qed.
+
+Lemma eq_unalltaus_eq (t s : itree E R) t'
+    (UNTAUS : unalltausF (observe t) (observe t'))
+    (EQV: t ≅ s) :
+  exists s', unalltausF (observe s) (observe s') /\ t' ≅ s'.
+Proof.
+  eapply eq_unalltaus_eqF in UNTAUS; try eassumption.
+  destruct UNTAUS as [os' []]. eexists (go os'); split; eauto.
+  pfold. eapply eq_itreeF'_mono; eauto.
+Qed.
+
+(* Reflexivity of [eutt_0], modulo a few assumptions. *)
+Lemma reflexive_euttF0 I (eutt : relation I) ot :
+  Reflexive eutt -> notauF ot -> eq_notauF eutt ot ot.
+Proof.
+  intros. destruct ot; try contradiction; econstructor; intros; subst; eauto.
+Qed.
+
+Lemma euttF_tau r t1 t2 t1' t2'
+    (OBS1: TauF t1' = observe t1)
+    (OBS2: TauF t2' = observe t2)
+    (REL: eutt_ r t1' t2'):
+  eutt_ r t1 t2.
+Proof.
+  intros. destruct REL. econstructor.
+  - simpobs. rewrite !finite_taus_tau. eauto.
+  - intros. eapply EQV; eapply unalltaus_tau; eauto.
+Qed.
+
+Lemma euttF_tau_left r t1 t2 t1'
+    (OBS: TauF t1 = observe t1')
+    (REL: eutt_ r t1' t2):
+  eutt_ r t1 t2.
+Proof.
+  intros. destruct REL. econstructor.
+  - rewrite <- FIN. symmetry. rewrite <- OBS. rewrite <- finite_taus_tau; eauto. reflexivity.
+  - intros. eapply EQV; eauto. rewrite <- OBS. inversion UNTAUS1. constructor; auto.
+    econstructor; eauto.
+Qed.
+
+Lemma euttF_tau_right r t1 t2 t2'
+    (OBS: TauF t2 = observe t2')
+    (REL: eutt_ r t1 t2'):
+  eutt_ r t1 t2.
+Proof.
+  intros. destruct REL. econstructor.
+  - rewrite FIN. rewrite <- OBS. rewrite <- finite_taus_tau; eauto. reflexivity.
+  - intros. eapply EQV; eauto. rewrite <- OBS. inversion UNTAUS2. constructor; auto.
+    econstructor; eauto.
+Qed.
+
+Lemma euttF_vis {u} (r : relation (itree E R)) t1 t2 (e : _ u) k1 k2
+    (OBS1: VisF e k1 = observe t1)
+    (OBS2: VisF e k2 = observe t2)
+    (REL: forall x, r (k1 x) (k2 x)):
+  eutt_ r t1 t2.
+Proof.
+  intros. econstructor.
+  - split; intros; eapply notau_finite_taus; eauto.
+  - intros.
+    apply unalltaus_notau_id in UNTAUS1; eauto.
+    apply unalltaus_notau_id in UNTAUS2; eauto.
+    simpobs. subst. eauto.
+Qed.
+
+(**)
+
+Lemma Reflexive_euttF (r : relation (itree E R)) :
+  Reflexive r -> Reflexive (euttF r).
+Proof.
+  split.
+  - reflexivity.
+  - intros.
+    erewrite (unalltaus_injective _ _ _ UNTAUS1 UNTAUS2).
+    apply reflexive_euttF0; eauto using unalltaus_notau.
+Qed.
+
+Lemma eutt_refl r x : paco2 eutt_ r x x.
+Proof.
+  revert x. pcofix CIH.
+  intros. pfold. apply Reflexive_euttF. eauto.
+Qed.
+
+(* [eutt] is an equivalence relation. *)
+Global Instance Reflexive_eutt: (Reflexive eutt).
+Proof.
+  repeat intro. apply eutt_refl.
+Qed.
+
+Global Instance Symmetric_eutt
+: Symmetric eutt.
+Proof.
+  pcofix Symmetric_eutt.
+  intros t1 t2 H12.
+  punfold H12.
+  pfold.
+  destruct H12 as [I12 H12].
+  split.
+  - symmetry; assumption.
+  - intros. hexploit H12; eauto. intros.
+    inv H; eauto.
+    econstructor. intros. specialize (H0 x). pclearbot. eauto.
+Qed.
+
+Global Instance Transitive_eutt : Transitive eutt.
+Proof.
+  pcofix Transitive_eutt.
+  intros t1 t2 t3 H12 H23.
+  punfold H12.
+  punfold H23.
+  pfold.
+  destruct H12 as [I12 H12].
+  destruct H23 as [I23 H23].
+  split.
+  - etransitivity; eauto.
+  - intros t1' t3' H1 H3.
+    destruct I12 as [I1 I2].
+    destruct I1 as [n2' [t2' TAUS2]]; eauto.
+    hexploit H12; eauto. intros REL1.
+    hexploit H23; eauto. intros REL2.
+    destruct REL1; inversion REL2; clear REL2; eauto.
+    auto_inj_pair2; subst.
+    econstructor. intros.
+    specialize (H x); specialize (H6 x). pclearbot. eauto.
+Qed.
+
+(**)
+
+(* [eutt] is preserved by removing one [Tau]. *)
+Lemma tauF_eutt (t t': itree E R) (OBS: TauF t' = observe t): t ~~ t'.
+Proof.
+  pfold. split.
+  - simpobs. rewrite finite_taus_tau. reflexivity.
+  - intros t1' t2' H1 H2.
+    eapply unalltaus_tau in H1; eauto.
+    assert (X := unalltaus_injective _ _ _ H1 H2).
+    subst; apply reflexive_euttF0; eauto using unalltaus_notau.
+    left. apply Reflexive_eutt.
+Qed.
+
+Lemma tau_eutt (t: itree E R) : Tau t ~~ t.
+Proof.
+  eapply tauF_eutt. eauto.
+Qed.
+
+(* [eutt] is preserved by removing all [Tau]. *)
+Lemma untaus_eutt (t t' : itree E R) : untausF (observe t) (observe t') -> t ~~ t'.
+Proof.
+  intros H.
+  pfold. split.
+  - eapply untaus_finite_taus; eauto.
+  - induction H; intros.
+    + rewrite (unalltaus_injective _ _ _ UNTAUS1 UNTAUS2).
+      apply reflexive_euttF0; eauto using unalltaus_notau.
+      left; apply Reflexive_eutt.
+    + eapply unalltaus_tau in UNTAUS1; eauto.
+Qed.
+
+End EUTT.
+
+Hint Constructors eq_notauF.
+Hint Constructors eq_notauF'.
+Hint Constructors untausF.
+Hint Unfold unalltausF.
+Hint Unfold finite_tausF.
+Hint Constructors euttF.
+Hint Resolve monotone_eutt_ : paco.
+Hint Resolve notau_ret.
+Hint Resolve notau_vis.
+Hint Resolve notau_tau.
+
+Delimit Scope eutt_scope with eutt.
+
+Infix "~~" := eutt (at level 70).
+
+Notation finite_taus t := (finite_tausF (observe t)).
+Notation untaus t t' := (untausF (observe t) (observe t')).
+Notation unalltaus t t' := (unalltausF (observe t) (observe t')).
+
+(* We can now rewrite with [eutt] equalities. *)
+Instance Equivalence_eutt E R : @Equivalence (itree E R) eutt.
+Proof. constructor; typeclasses eauto. Qed.
+
+Instance subrelation_eq_eutt {E R} : subrelation (@eq_itree E R) eutt.
+Proof.
+  pcofix CIH. intros.
+  pfold. econstructor.
+  { split; [|symmetry in H0]; intros; destruct H as [n [? ?]]; eauto using eq_unalltaus. }
+
+  intros. eapply eq_unalltaus_eqF in H0; eauto. destruct H0 as [s' [UNTAUS' EQV']].
+  hexploit @unalltaus_injective; [apply UNTAUS' | apply UNTAUS2 | intro X]; subst.
+  inv EQV'; simpobs; eauto.
+  eapply unalltaus_notau in UNTAUS1. simpobs. contradiction.
+Qed.
+
+Instance subrelation_go_sim_eq_eutt {E R} : subrelation (go_sim (@eq_itree E R)) (go_sim (@eutt E R)).
+Proof.
+  repeat intro. red. red in H. rewrite H. reflexivity.
+Qed.
+
+Instance eutt_go {E R} :
+  Proper (go_sim (@eutt E R) ==> @eutt E R) (@go E R).
+Proof.
+  repeat intro. eauto.
+Qed.
+
+Instance eutt_observe {E R} :
+  Proper (@eutt E R ==> go_sim (@eutt E R)) (@observe E R).
+Proof.
+  repeat intro. punfold H. pfold. destruct H. econstructor; eauto.
+Qed.
+
+Instance eutt_tauF {E R} :
+  Proper (@eutt E R ==> go_sim (@eutt E R)) (@TauF E R _).
+Proof.
+  repeat intro. pfold. punfold H.
+  destruct H. econstructor.
+  - split; intros; simpl.
+    + rewrite finite_taus_tau, <-FIN, <-finite_taus_tau; eauto.
+    + rewrite finite_taus_tau, FIN, <-finite_taus_tau; eauto.
+  - intros. eapply EQV; eapply unalltaus_tau; eauto.
+Qed.
+
+Instance eutt_VisF {E R u} (e: E u) :
+  Proper (pointwise_relation _ eutt ==> go_sim (@eutt E R)) (VisF e).
+Proof.
+  repeat intro. red in H. pfold. econstructor.
+  - repeat econstructor.
+  - intros.
+    destruct UNTAUS1 as [UNTAUS1 Hnotau1].
+    destruct UNTAUS2 as [UNTAUS2 Hnotau2].
+    dependent destruction UNTAUS1.
+    dependent destruction UNTAUS2. simpobs.
+    econstructor; intros; left; apply H.
+Qed.
+
+Instance eq_itree_notauF {E R} :
+  Proper (go_sim (@eq_itree E R) ==> flip impl) (@notauF E R _).
+Proof.
+  repeat intro. punfold H. inv H; simpl in *; subst; eauto.
+Qed.
+
+(* If [t1] and [t2] are equivalent, then either both start with
+   finitely many taus, or both [spin]. *)
+Instance eutt_finite_taus {E R} :
+  Proper (go_sim (@eutt E R) ==> flip impl) (@finite_tausF E R).
+Proof.
+  repeat intro. punfold H. eapply H. eauto.
+Qed.
+
+(* Lemmas about [bind]. *)
+
+Lemma untaus_bind {E S R} : forall t t' (k: S -> itree E R)
+      (UNTAUS: untausF (observe t) (observe t')),
+  untausF (observe (ITree.bind t k)) (observe (ITree.bind t' k)).
+Proof.
+  intros. genobs t ot; genobs t' ot'. revert t Heqot t' Heqot'.
+  induction UNTAUS; intros; subst.
+  - rewrite !bind_unfold; simpobs; eauto.
+  - rewrite bind_unfold. simpobs. cbn. eauto.
+Qed.
+
+Lemma untaus_bindF {E S R} : forall t t' (k: S -> itree E R)
+      (UNTAUS: untausF (observe t) t'),
+  untausF (observe (ITree.bind t k)) (observe (ITree.bind (go t') k)).
+Proof.
+  intros; eapply untaus_bind; eauto.
+Qed.
+
+Lemma finite_taus_bind_fst {E R S}
+      (t : itree E R) (f : R -> itree E S) :
+  finite_taus (ITree.bind t f) -> finite_taus t.
+Proof.
+  intros [tf' [TAUS PROP]].
+  genobs (ITree.bind t f) obtf. move TAUS at top. revert_until TAUS.
+  induction TAUS; intros; subst.
+  - rewrite bind_unfold in PROP.
+    genobs t ot; destruct ot; eauto using finite_taus_ret, finite_taus_vis.
+  - genobs t ot; destruct ot; eauto using finite_taus_ret, finite_taus_vis.
+    rewrite bind_unfold in Heqobtf. simpobs. inv Heqobtf. unfold_bind.
+    eapply finite_taus_tau; eauto.
+Qed.
+
+Lemma finite_taus_bind {E R S}
+      (t : itree E R) (f : R -> itree E S)
+      (FINt: finite_tausF (observe t))
+      (FINk: forall v, finite_tausF (observe (f v))):
+  finite_tausF (observe (ITree.bind t f)).
+Proof.
+  rewrite bind_unfold.
+  genobs t ot. clear Heqot t.
+  destruct FINt as [ot' [UNT NOTAU]].
+  induction UNT; subst.
+  - destruct ot0; inv NOTAU; simpl; eauto 7.
+  - apply finite_taus_tau. eauto.
+Qed.
+
+Lemma untaus_eq_idx E R: forall (ot1 ot2: itreeF E R _),
+    untausF ot1 ot2 -> untausF ot1 ot2.
+Proof. intros; subst; eauto. Qed.
+
+Lemma untaus_untaus E R: forall (ot1 ot2 ot3: itreeF E R _),
+    untausF ot1 ot2 -> untausF ot2 ot3 -> untausF ot1 ot3.
+Proof.
+  intros t1 t2 t3. induction 1; simpl; eauto.
+Qed.
+
+Lemma untaus_unalltus_rev E R (ot1 ot2 ot3: itreeF E R _) :
+    untausF ot1 ot2 -> unalltausF ot1 ot3 -> unalltausF ot2 ot3.
+Proof.
+  intros H. revert ot3.
+  induction H; intros.
+  - eauto using untaus_eq_idx with arith.
+  - destruct H0 as [Huntaus Hnotau].
+    destruct Huntaus.
+    + exfalso; eauto.
+    + inv OBS0. inversion H0; subst; eauto.
+Qed.
+
+Lemma eutt_strengthen {E R}:
+  forall r (t1 t2: itree E R)
+     (FIN: finite_taus t1 <-> finite_taus t2)
+     (EQV: forall t1' t2'
+              (UNT1: unalltaus t1 t1')
+              (UNT2: unalltaus t2 t2'),
+         paco2 (eutt_ ∘ gres2 eutt_) r t1' t2'),
+    paco2 (eutt_ ∘ gres2 eutt_) r t1 t2.
+Proof.
+  intros. pfold. econstructor; eauto.
+  intros.
+  hexploit (EQV (go ot1') (go ot2')); eauto.
+  intros EQV'. punfold EQV'. destruct EQV'.
+  eapply EQV0;
+    repeat constructor; eauto. eapply UNTAUS1. eapply UNTAUS2.
+Qed.
+
+Inductive eutt_trans_clo {E R} (r: relation (itree E R)) : relation (itree E R) :=
+| eutt_pre_clo_intro (t1 t2 t3 t4: itree E R)
+      (EQVl: t1 ~~ t2)
+      (EQVr: t4 ~~ t3)
+      (REL: r t2 t3)
+  : eutt_trans_clo r t1 t4
+.
+Hint Constructors eutt_trans_clo.
+
+Lemma eutt_clo_trans E R: weak_respectful2 (@eutt_ E R) eutt_trans_clo.
+Proof.
+  econstructor; [pmonauto|].
+  intros. inv PR.
+  punfold EQVl. punfold EQVr. destruct EQVl, EQVr. split.
+  { rewrite FIN, FIN0. apply GF in REL. destruct REL. eauto. }
+
+  intros. apply proj1 in FIN. edestruct FIN as [n'' [t2'' TAUS'']]; [eexists; eauto|].
+  hexploit EQV; eauto. intros EUTT1.
+  apply proj1 in FIN0. edestruct FIN0 as [n''' [t2''' TAUS''']]; [eexists; eauto|].
+  hexploit EQV0; eauto. intros EUTT2.
+  apply GF in REL. destruct REL.
+  hexploit EQV1; eauto. intros EUTT3.
+  destruct EUTT1; destruct EUTT2;
+    try (solve [inversion EUTT3; auto]).
+  remember (VisF _ _) as o2 in EUTT3.
+  remember (VisF _ _) as o3 in EUTT3.
+  inversion EUTT3; subst; try discriminate.
+  inversion H2; clear H2; inversion H3; clear H3.
+  subst; auto_inj_pair2; subst.
+  econstructor. intros.
+  specialize (H x); specialize (H0 x); specialize (H1 x).
+  pclearbot. eauto using rclo2.
+Qed.
+
+Inductive eutt_bind_clo {E R} (r: relation (itree E R)) : relation (itree E R) :=
+| eutt_bind_clo_intro U (t1 t2: itree E U) k1 k2
+      (EQV: t1 ~~ t2)
+      (REL: forall v, r (k1 v) (k2 v))
+  : eutt_bind_clo r (ITree.bind t1 k1) (ITree.bind t2 k2)
+.
+Hint Constructors eutt_bind_clo.
+
+Lemma bind_clo_finite_taus E U R (t1 t2: itree E U) (k1 k2: U -> itree E R)
+    (FT: finite_taus (ITree.bind t1 k1))
+    (FTk: forall v, finite_taus (k1 v) -> finite_taus (k2 v))
+    (EQV: t1 ~~ t2):
+  finite_taus (ITree.bind t2 k2).
+Proof.
+  punfold EQV. destruct EQV as [[FTt _] EQV].
+  assert (FT1 := FT). apply finite_taus_bind_fst in FT1.
+  assert (FT2 := FT1). apply FTt in FT2.
+  destruct FT1 as [a [FT1 NT1]], FT2 as [b [FT2 NT2]].
+  rewrite @untaus_finite_taus in FT; [|eapply untaus_bindF, FT1].
+  rewrite bind_unfold. genobs t2 ot2. clear Heqot2 t2.
+  induction FT2.
+  - destruct ot0; inv NT2; simpl; eauto 7.
+    hexploit EQV; eauto. intros EQV'. inv EQV'.
+    rewrite bind_unfold in FT. eauto.
+  - subst. eapply finite_taus_tau; eauto.
+    eapply IHFT2; eauto using unalltaus_tau'.
+Qed.
+
+Lemma eutt_clo_bind E R: weak_respectful2 (@eutt_ E R) eutt_bind_clo.
+Proof.
+  econstructor; [pmonauto|].
+  intros. destruct PR. split.
+  - assert (EQV':=EQV). symmetry in EQV'.
+    split; intros; eapply bind_clo_finite_taus; eauto; intros.
+    + edestruct GF; eauto. apply FIN. eauto.
+    + edestruct GF; eauto. apply FIN. eauto.
+  - punfold EQV. destruct EQV.
+    intros.
+    hexploit (@finite_taus_bind_fst E); [do 2 eexists; apply UNTAUS1|]. intros [a FT1].
+    hexploit (@finite_taus_bind_fst E); [do 2 eexists; apply UNTAUS2|]. intros [b FT2].
+    specialize (EQV _ _ FT1 FT2).
+    destruct FT1 as [FT1 Hnotau1]. destruct FT2 as [FT2 Hnotau2].
+    hexploit @untaus_bindF; [ eapply FT1 | ]. intros UT1.
+    hexploit @untaus_bindF; [ eapply FT2 | ]. intros UT2.
+    hexploit untaus_unalltus_rev; [apply UT1| |]. eauto. intros UAT1.
+    hexploit untaus_unalltus_rev; [apply UT2| |]; eauto. intros UAT2.
+    inv EQV.
+    + rewrite bind_unfold in UAT1, UAT2. simpobs. cbn in *.
+      eapply GF in REL. destruct REL.
+      eapply monotone_eq_notauF; eauto using rclo2.
+    + rewrite bind_unfold in UAT1, UAT2. simpobs. cbn in *.
+      destruct UAT1 as [UAT1 _]. destruct UAT2 as [UAT2 _].
+      dependent destruction UAT1. dependent destruction UAT2. simpobs.
+      econstructor. intros. specialize (H x). pclearbot. fold_bind. eauto using rclo2.
+Qed.
+
+(* [eutt] is a congruence wrt. [bind] *)
+
+Instance eutt_bind {E R S} :
+  Proper (@eutt E R ==>
+          pointwise_relation _ eutt ==>
+          @eutt E S) ITree.bind.
+Proof.
+  repeat intro. pupto2_init.
+  pupto2 eutt_clo_bind. econstructor; eauto.
+  intros. pupto2_final. apply H0.
+Qed.
+
+Instance eutt_paco {E R} r:
+  Proper (@eutt E R ==> @eutt E R ==> flip impl)
+         (paco2 (eutt_ ∘ gres2 eutt_) r).
+Proof.
+  repeat intro. pupto2 eutt_clo_trans. eauto.
+Qed.
+
+Instance eutt_gres {E R} r:
+  Proper (@eutt E R ==> @eutt E R ==> flip impl)
+         (gres2 eutt_ r).
+Proof.
+  repeat intro. pupto2 eutt_clo_trans. eauto.
+Qed.
+
+Instance eutt_map {E R S} :
+  Proper (pointwise_relation _ eq ==> @eutt E R ==> @eutt E S) ITree.map.
+Proof.
+Admitted.
+
+Instance eutt_forever {E R S} :
+  Proper (@eutt E R ==> @eutt E S) ITree.forever.
+Proof.
+Admitted.
+Instance eutt_when {E} (b : bool) :
+  Proper (@eutt E unit ==> @eutt E unit) (ITree.when b).
+Proof.
+Admitted.
+
+Lemma eutt_map_map {E R S T}
+      (f : R -> S) (g : S -> T) (t : itree E R) :
+  eutt (ITree.map g (ITree.map f t))
+       (ITree.map (fun x => g (f x)) t).
+Proof.
+  rewrite map_map. reflexivity.
+Qed.
+
+Notation itree' E R := (itreeF E R (itree E R)).
+
+Definition observing {E R}
+           (f : itree' E R -> itree' E R -> Prop)
+           (x y : itree E R) :=
+  f x.(observe) y.(observe).
+
+Inductive euttF1' {E R} (r : itree E R -> itree E R -> Prop) :
+  itree' E R -> itree' E R -> Prop :=
+| euttF1_Tau_L : forall t1 t2,
+    euttF1' r t1.(observe) t2 ->
+    euttF1' r (TauF t1) t2
+| euttF1_Tau_R : forall t1 t2,
+    euttF1' r t1 t2.(observe) ->
+    euttF1' r t1 (TauF t2)
+| euttF1_euttF0 : forall t1 t2,
+    eq_notauF r t1 t2 ->
+    euttF1' r t1 t2
+.
+
+Definition euttF1 {E R} (r : relation (itree E R)) :
+  relation (itree E R) := observing (euttF1' r).
+
+Lemma euttF1_euttF {E R} (r : relation (itree E R)) :
+  forall t1 t2,
+    euttF1 r t1 t2 -> eutt_ r t1 t2.
+Proof.
+Admitted.
+
+Inductive euttF' {E R} (eutt: relation (itree E R)) (eqtaus: relation (itreeF E R _))
+  : relation (itreeF E R _) :=
+| euttF'_ret r : euttF' eutt eqtaus (RetF r) (RetF r)
+| euttF'_vis u (e : E u) k1 k2
+      (EUTTK: forall x, eutt (k1 x) (k2 x)):
+    euttF' eutt eqtaus (VisF e k1) (VisF e k2)
+| euttF'_tau_tau t1 t2
+      (EQTAUS: eqtaus (observe t1) (observe t2)):
+    euttF' eutt eqtaus (TauF t1) (TauF t2)
+| euttF'_tau_left t1 ot2
+      (EQTAUS: euttF' eutt eqtaus (observe t1) ot2):
+    euttF' eutt eqtaus (TauF t1) ot2
+| euttF'_right ot1 t2
+      (EQTAUS: euttF' eutt eqtaus ot1 (observe t2)):
+    euttF' eutt eqtaus ot1 (TauF t2)
+.
+Hint Constructors euttF'.
+
+Definition eutt'_ {E R} eutt t1 t2 := paco2 (@euttF' E R eutt) bot2 (* (fun x y => eutt (go x) (go y)) *) (observe t1) (observe t2).
+Hint Unfold eutt'_.
+
+Definition eutt' {E R} := paco2 (@eutt'_ E R) bot2.
+Hint Unfold eutt'.
+
+Lemma euttF'_mon {E R} r r' s s' x y
+    (EUTT: @euttF' E R r s x y)
+    (LEr: r <2= r')
+    (LEs: s <2= s'):
+  euttF' r' s' x y.
+Proof.
+  induction EUTT; eauto.
+Qed.
+
+Lemma monotone_euttF' {E R} eutt : monotone2 (@euttF' E R eutt).
+Proof. repeat intro. eauto using euttF'_mon. Qed.
+Hint Resolve monotone_euttF' : paco.
+
+Lemma monotone_eutt'_ {E R} : monotone2 (@eutt'_ E R).
+Proof. red. eauto using euttF'_mon, paco2_mon_gen. Qed.
+Hint Resolve monotone_eutt'_ : paco.
+
+Lemma eutt__is_eutt'_ {E R} r (t1 t2: itree E R) :
+  eutt_ r t1 t2 <-> eutt'_ r t1 t2.
+Proof.
+  split; intros.
+  { revert t1 t2 H. pcofix CIH'. intros. destruct H0.
+    genobs t1 ot1. genobs t2 ot2. clear Heqot1 t1 Heqot2 t2.
+    assert (EM: notauF ot1 \/ notauF ot2 \/ ~(notauF ot1 \/ notauF ot2))
+      by (destruct ot1, ot2; simpl; tauto).
+    destruct EM as [EM|[EM|EM]].
+    - destruct FIN as [FIN _].
+      hexploit FIN; eauto 7. clear FIN; intro FIN.
+      destruct FIN as [ot' [UNTAUS NOTAU]].
+      hexploit EQV; eauto. intros EQNT.
+      induction UNTAUS; subst.
+      { pfold. inv EQNT; eauto. }
+      hexploit IHUNTAUS; eauto.
+      { intros. destruct UNTAUS1.
+        dependent destruction H; [|subst; contradiction].
+        hexploit @unalltaus_injective; [|econstructor|]; eauto. intros; subst; eauto.
+      }
+      intros EUTT. punfold EUTT.
+    - destruct FIN as [_ FIN].
+      hexploit FIN; eauto 7. clear FIN; intro FIN.
+      destruct FIN as [ot' [UNTAUS NOTAU]].
+      hexploit EQV; eauto. intros EQNT.
+      induction UNTAUS; subst.
+      { pfold. inv EQNT; eauto. }
+      hexploit IHUNTAUS; eauto.
+      { intros. destruct UNTAUS2.
+        dependent destruction H; [|subst; contradiction].
+        hexploit @unalltaus_injective; [|econstructor|]; eauto. intros; subst; eauto.
+      }
+      intros EUTT. punfold EUTT.
+    - destruct ot1, ot2; simpl in *; try tauto.
+      pfold. econstructor. right. apply CIH'.
+      econstructor.
+      + rewrite !finite_taus_tau in FIN. eauto.
+      + eauto using unalltaus_tau'.
+  }
+  { punfold H. econstructor; intros.
+    - split; intros.
+      + genobs t1 ot1. genobs t2 ot2. clear Heqot1 t1 Heqot2 t2.
+        destruct H0 as [ot' [UNTAUS NOTAU]].
+        move UNTAUS before r. revert_until UNTAUS.
+        induction UNTAUS; intros.
+        * induction H; eauto; try contradiction.
+          rewrite finite_taus_tau. eauto.
+        * induction H; eauto 7; try inv OBS; pclearbot
+          ; rewrite ?finite_taus_tau; eauto; eapply IHUNTAUS; eauto.
+          punfold EQTAUS.
+     + genobs t1 ot1. genobs t2 ot2. clear Heqot1 t1 Heqot2 t2.
+       destruct H0 as [ot' [UNTAUS NOTAU]].
+       move UNTAUS before r. revert_until UNTAUS.
+       induction UNTAUS; intros.
+       * induction H; eauto; try contradiction.
+         rewrite finite_taus_tau. eauto.
+       * induction H; eauto 7; try inv OBS; pclearbot
+         ; rewrite ?finite_taus_tau; eauto; eapply IHUNTAUS; eauto.
+         punfold EQTAUS.
+    - genobs t1 ot1. genobs t2 ot2. clear Heqot1 t1 Heqot2 t2.
+      destruct UNTAUS1 as [UNTAUS1 NT1]. destruct UNTAUS2 as [UNTAUS2 NT2].
+      move UNTAUS2 before r. move UNTAUS1 before r. revert_until UNTAUS1.
+      induction UNTAUS1.
+      + induction 1; intros.
+        * inv H; try contradiction; eauto.
+        * subst. inv H; try contradiction. eauto.
+      + induction 1; intros; subst.
+        * inv H; try contradiction; eauto.
+        * inv H; try contradiction; eauto.
+          pclearbot. eapply IHUNTAUS1; eauto.
+          punfold EQTAUS.
+  }
+Qed.
+
+Lemma eutt_is_eutt' {E R} r (t1 t2: itree E R) :
+  paco2 eutt_ r t1 t2 <-> paco2 eutt'_ r t1 t2.
+Proof.
+  split; intros; eapply paco2_mon_gen; eauto; intros; apply eutt__is_eutt'_; eauto.
+Qed.
+
+Lemma eutt_is_eutt'_gres {E R} r (t1 t2: itree E R) :
+  paco2 (eutt_ ∘ gres2 eutt_) r t1 t2 <-> paco2 (eutt'_ ∘ gres2 eutt'_) r t1 t2.
+Proof.
+  split; intros.
+  - eapply paco2_mon_gen; eauto. intros.
+    red in PR|-*. rewrite <-eutt__is_eutt'_.
+    eapply monotone_eutt_; eauto. intros.
+    eapply grespectful2_impl; eauto. intros.
+    rewrite eutt__is_eutt'_. reflexivity.
+  - eapply paco2_mon_gen; eauto. intros.
+    red in PR|-*. rewrite eutt__is_eutt'_.
+    eapply monotone_eutt'_; eauto. intros.
+    eapply grespectful2_impl; eauto. intros.
+    rewrite eutt__is_eutt'_. reflexivity.
+Qed.
+
+Instance eutt'_paco {E R} r:
+  Proper (@eutt E R ==> @eutt E R ==> flip impl)
+         (paco2 (eutt'_ ∘ gres2 eutt'_) r).
+Proof.
+  repeat intro.
+  rewrite <-eutt_is_eutt'_gres.
+  rewrite <-eutt_is_eutt'_gres in H1.
+  rewrite H, H0. eauto.
+Qed.
+
+Instance eutt'_gres {E R} r:
+  Proper (@eutt E R ==> @eutt E R ==> flip impl)
+         (gres2 eutt'_ r).
+Proof.
+  repeat intro.
+  rewrite grespectful2_iff; [|intros; erewrite eutt__is_eutt'_; reflexivity].
+  rewrite grespectful2_iff in H1; [|intros; erewrite eutt__is_eutt'_; reflexivity].
+  rewrite H, H0. eauto.
+Qed.
